Transform.v
@@ -1,0 +1,41 @@
+(* This file is part of the LLIR Semantics project. *)
+(* Licensing information is available in the LICENSE file. *)
+(* (C) 2020 Nandor Licker. All rights reserved. *)
+
+Require Import Coq.PArith.PArith.
+Require Import Coq.Lists.List.
+
+Require Import LLIR.Maps.
+Require Import LLIR.State.
+Require Import LLIR.Aliasing.
+Require Import LLIR.LLIR.
+Require Import LLIR.Verify.
+
+
+
+Definition rewrite_uses (i: inst) (f: reg -> reg): inst :=
+  match i with
+  | LLLd addr dst next => LLLd (f addr) dst next
+  | LLSt addr val next => LLSt (f addr) (f val) next
+  | LLArg index dst next => i
+  | LLConst value dst next => i
+  | LLFrame object dst next => i
+  | LLGlobal object dst next => i
+  | LLExtern id next => i
+  | LLInvoke t args dst next exn => LLInvoke (f t) (List.map f args) dst next exn
+  | LLRet value => LLRet (f value)
+  | LLJcc cond bt bf => LLJcc (f cond) bt bf
+  | LLJmp target => i
+  | LLUnop op arg dst next => LLUnop op (f arg) dst next
+  | LLBinop op lhs rhs dst next => LLBinop op (f lhs) (f rhs) dst next
+  end.
+
+
+Theorem use_rewritten:
+  forall (i: inst) (src: reg) (f: reg -> reg),
+    Uses i src -> Uses (rewrite_uses i f) (f src).
+Proof.
+  destruct i; intros src f Huse; simpl; inversion Huse; try rewrite H; auto.
+  right. apply List.in_map_iff. exists src.
+  split. reflexivity. apply H. 
+Qed.
